src/localdrfra/LocalDRFRA.v
@@ -1,0 +1,40 @@
+Require Import Omega.
+Require Import Bool.
+Require Import RelationClasses.
+
+From sflib Require Import sflib.
+From Paco Require Import paco.
+
+From PromisingLib Require Import Axioms.
+From PromisingLib Require Import Basic.
+From PromisingLib Require Import DataStructure.
+From PromisingLib Require Import DenseOrder.
+From PromisingLib Require Import Loc.
+From PromisingLib Require Import Language.
+
+Require Import Event.
+Require Import Time.
+Require Import View.
+Require Import Cell.
+Require Import Memory.
+Require Import TView.
+Require Import Local.
+Require Import Thread.
+Require Import Configuration.
+Require Import Behavior.
+
+Require Import OrdStep.
+Require Import Stable.
+Require Import RARace.
+Require Import RASimThread.
+
+Set Implicit Arguments.
+
+
+Theorem local_drf_ra
+        L s
+        (RACEFREE: RARace.racefree L s):
+  behaviors Configuration.step (Configuration.init s) <1=
+  behaviors (@OrdConfiguration.step L Ordering.acqrel) (Configuration.init s).
+Proof.
+Admitted.
