src/localdrfra/RARace.v
@@ -1,0 +1,108 @@
+Require Import Omega.
+Require Import Bool.
+Require Import RelationClasses.
+
+From sflib Require Import sflib.
+From Paco Require Import paco.
+
+From PromisingLib Require Import Axioms.
+From PromisingLib Require Import Basic.
+From PromisingLib Require Import DataStructure.
+From PromisingLib Require Import DenseOrder.
+From PromisingLib Require Import Loc.
+From PromisingLib Require Import Language.
+
+Require Import Event.
+Require Import Time.
+Require Import View.
+Require Import Cell.
+Require Import Memory.
+Require Import TView.
+Require Import Local.
+Require Import Thread.
+Require Import Configuration.
+
+Require Import OrdStep.
+
+
+Module ReleaseWrites.
+  Definition t: Type := list (Loc.t * Time.t).
+
+  Definition rel_write (e: ThreadEvent.t): option (Loc.t * Time.t) :=
+    match e with
+    | ThreadEvent.write loc from to val released ord =>
+      if Ordering.le Ordering.acqrel ord then Some (loc, to) else None
+    | ThreadEvent.update loc tsr to valr valw releasedr releasedw ordr ordw =>
+      if Ordering.le Ordering.acqrel ordw then Some (loc, to) else None
+    | _ => None
+    end.
+
+  Definition append (rels: t) (e: ThreadEvent.t): t :=
+    match rel_write e with
+    | Some r => r :: rels
+    | None => rels
+    end.
+End ReleaseWrites.
+
+
+Module RARace.
+  Section RARace.
+    Variable L: Loc.t -> bool.
+
+    Inductive thread_steps lang: forall (rels: ReleaseWrites.t) (e1 e2: Thread.t lang), Prop :=
+    | thread_steps_refl
+        e:
+        thread_steps lang [] e e
+    | thread_steps_step
+        rels pf e e1 e2 e3
+        (STEPS: @thread_steps lang rels e1 e2)
+        (STEP: @OrdThread.step lang L Ordering.acqrel pf e e2 e3)
+        (SILENT: ThreadEvent.get_machine_event e = MachineEvent.silent):
+        thread_steps lang (ReleaseWrites.append rels e) e1 e3
+    .
+
+    Inductive configuration_step: forall (e: MachineEvent.t) (tid: Ident.t) (rels: ReleaseWrites.t) (c1 c2: Configuration.t), Prop :=
+    | configuration_step_intro
+        rels
+        pf e tid c1 lang st1 lc1 e2 st3 lc3 sc3 memory3
+        (TID: IdentMap.find tid c1.(Configuration.threads) = Some (existT _ lang st1, lc1))
+        (STEPS: thread_steps lang rels (Thread.mk _ st1 lc1 c1.(Configuration.sc) c1.(Configuration.memory)) e2)
+        (STEP: OrdThread.step L Ordering.acqrel pf e e2 (Thread.mk _ st3 lc3 sc3 memory3))
+        (CONSISTENT: OrdThread.consistent L Ordering.acqrel (Thread.mk _ st3 lc3 sc3 memory3)):
+        configuration_step (ThreadEvent.get_machine_event e) tid (ReleaseWrites.append rels e)
+                           c1 (Configuration.mk (IdentMap.add tid (existT _ _ st3, lc3) c1.(Configuration.threads)) sc3 memory3)
+    .
+
+    Inductive configuration_steps: forall (rels: ReleaseWrites.t) (c1 c2: Configuration.t), Prop :=
+    | configuration_steps_refl
+        c:
+        configuration_steps [] c c
+    | configuration_steps_step
+        rels e tid rels' c1 c2 c3
+        (STEPS: configuration_steps rels c1 c2)
+        (STEP: configuration_step e tid rels' c2 c3):
+        configuration_steps (rels' ++ rels) c1 c3
+    .
+
+
+    (* race condition *)
+
+    Definition ra_race (rels: ReleaseWrites.t) (tview: TView.t) (loc: Loc.t) (to: Time.t) (ordr: Ordering.t): Prop :=
+      <<LOC: L loc>> /\
+      <<HIGHER: Time.lt (tview.(TView.cur).(View.rlx) loc) to>> /\
+      (<<ORDW: ~ List.In (loc, to) rels>> \/
+       <<ORDR: Ordering.le ordr Ordering.strong_relaxed>>).
+
+    Definition racefree (s: Threads.syntax): Prop :=
+      forall rels c
+        tid lang st1 lc1
+        pf loc to val released ord e2 e3
+        (CSTEPS: configuration_steps rels (Configuration.init s) c)
+        (TID: IdentMap.find tid c.(Configuration.threads) = Some (existT _ lang st1, lc1))
+        (STEPS: rtc (@OrdThread.tau_step lang L Ordering.acqrel)
+                    (Thread.mk _ st1 lc1 c.(Configuration.sc) c.(Configuration.memory)) e2)
+        (STEP: OrdThread.step L Ordering.acqrel pf (ThreadEvent.read loc to val released ord) e2 e3)
+        (RACE: ra_race rels e2.(Thread.local).(Local.tview) loc to ord),
+        False.
+  End RARace.
+End RARace.
